Makefile
@@ -48,7 +48,6 @@ COQSRCLIBS?=-I $(COQLIB)kernel -I $(COQLIB)lib \
   -I $(COQLIB)plugins/firstorder \
   -I $(COQLIB)plugins/fourier \
   -I $(COQLIB)plugins/funind \
-  -I $(COQLIB)plugins/interface \
   -I $(COQLIB)plugins/micromega \
   -I $(COQLIB)plugins/nsatz \
   -I $(COQLIB)plugins/omega \
